\documentclass{amsart}

\begin{document}

Kaiser Coadds, including w/o resampling

\begin{align}
\widetilde{\Psi}[r] =
\sum_{j=0}^{j<N}
\frac{\tau_j}{V_j}
\,
\widetilde{z}_j[r]
\,
\widetilde{\phi}_j[r]
\end{align}

\begin{align}
\widetilde{\Phi}[r]
=
\sum_{j=0}^{j<N}
\frac{\tau_j^2}{V_j}
\,
\left|
\widetilde{\phi}_j[r]
\right|^2
\end{align}

\begin{align}
\Psi[\mu] =
\sum_{j=0}^{j<N}
\frac{\tau_j}{V_j}
\sum_{x_j \in E_j}
z_j[x_j]
\,
\phi_j(A_j(x_j) - \mu)
\end{align}

\begin{align}
V_C = \left[
  \sum_{r \in \widetilde{C}}
  \sqrt{\widetilde{\Phi}[r]}
\right]^{-2}
\end{align}

\begin{align}
\widetilde{\phi}_C[r] =
\sqrt{V_C \, \widetilde{\Phi}[r]}
\end{align}

\begin{align}
\widetilde{z}_C[r] =
\frac{
  V_C \, \widetilde{\Psi}[r]
}{
  \widetilde{\phi}_C[r]
}
\end{align}

\begin{align}
\widetilde{K}_j[r] =
\frac{
  \widetilde{\phi}_j[r]
}{
  \widetilde{\phi}_C[r]
}
\end{align}

\begin{align}
z_C[\mu] = \sum_{j=0}^{j<N}
  \frac{\tau_j\,V_C}{V_j}
  \sum_{\eta \in C}
  K_j[\mu - \eta]
  \,
  z_j[\eta]
\end{align}


Sub-band Kaiser coadds

\begin{align}
\Psi_{\lambda}[\mu] =
    \sum_{j=0}^{j < N}
    \frac{\tau_{j,\lambda}}{V_j}
    \sum_{x_j \in E_j}
    z_j[x_j]
    \; \phi_{j,\lambda}\!\left(
        A_j(x_j) - \mu
    \right)
\end{align}

\begin{align}
\widetilde{\Phi}_{\lambda_1,\lambda_2}[r] =
    \sum_{j}
    \frac{
        \tau_{j,\lambda_1}
        \tau_{j,\lambda_2}
    }{
        V_j
    }
    \sum_{x_j}
    \widetilde{\phi}^*_{j,\lambda_1}\!(r)
    \;
    \widetilde{\phi}_{j,\lambda_2}\!(r)
\end{align}

\begin{align}
F_{\lambda,\lambda} =
\left[\sum_{r \in \widetilde{C}}
    \sqrt{\widetilde{\Phi}_{\lambda,\lambda}[r]}
\right]^2
\end{align}


\begin{align}
\widetilde{\phi}_{C,\lambda}[r] =
\sqrt{
    \frac{
        \widetilde{\Phi}_{\lambda,\lambda}[r]
    } {
        F_{\lambda,\lambda}
    }
}
\end{align}

\begin{align}
    F_{\lambda_1,\lambda_2}
    =
    \frac{
        \widetilde{\Phi}_{\lambda_1,\lambda_2}[r]
    }{
        \widetilde{\phi}^*_{C,\lambda_1}[r]
        \;
        \widetilde{\phi}_{C,\lambda_2}[r]
    }
\end{align}

\begin{align}
\widetilde{z}_{C,\lambda_1}[r]
= \sum_{\lambda_2}
F^{-1}_{\lambda_1,\lambda_2}
\frac{
    \widetilde{\Psi}_{\lambda_2}[r]
}{
    \widetilde{\phi}^*_{C,\lambda_2}[r]
}
\end{align}


Bad pixel interpolation

\begin{align}
\Psi[\mu] =
\sum_{j=0}^{j<N}
\frac{\tau_j}{V_j}
\sum_{x_j \in {G}_j}
z_j[x_j]
\;
\phi_{j}\!\left( A_j(x_j) - \mu \right)
\end{align}

\begin{align}
\Phi[\mu,\nu] =
\sum_{j=0}^{j<N}
\frac{\tau_j^2}{V_j}
\left[
\sum_{x_j \in {G}_j \cup {B}_j}
\phi_{j}\!\left( A_j(x_j) - \mu \right)
\,
\phi_{j}\!\left( A_j(x_j) - \nu \right)
\right.
\\
\quad\quad
\left.
-
\sum_{x_j \in {B}_j}
\phi_{j}\!\left( A_j(x_j) - \mu \right)
\,
\phi_{j}\!\left( A_j(x_j) - \nu \right)
\right]
\end{align}

\begin{align}
\widetilde{\Phi}[r, s]
=
\widetilde{\phi}^*_C[r]
\,
\widetilde{H}[r,s]
\,
\widetilde{\phi}_C[s]
\end{align}
\begin{align}
H[\mu,\nu]
= \frac{\delta[\mu-\nu]}{V_C} -
\sum_{j=0}^{j<N}
\frac{\tau_j^2}{V_j}
\sum_{x_j \in {B}_j}
K_{j}\!\left( A_j(x_j) - \mu \right)
\,
K_{j}\!\left( A_j(x_j) - \nu \right)
\end{align}

\begin{align}
\Psi[\mu] =
\sum_{\eta \in C}
\sum_{\nu \in C}
\phi_C[\eta - \mu]
\,
H[\eta,\nu]
\,
z_C[\nu]
\end{align}

\begin{align}
y[\mu]
=
\sum_{\nu \in C}
H[\mu,\nu]
\,
z_C[\nu]
\end{align}

\begin{align}
\mathbf{y}
= (\mathbf{V}_C^{-1} - \mathbf{R})
\mathbf{z}_C
\end{align}

\begin{align}
\widetilde{y}[r]
=
\frac{\widetilde{\Psi}[r]}{\widetilde{\phi}_C[r]}
\end{align}

\begin{align}
\mathbf{z}_C^{(k+1)}
=\mathbf{V}_C \left(
    \mathbf{y}
  + \mathbf{R}
  \,\mathbf{z}_C^{(k)}\right)
\end{align}

\begin{align}
\sum_{\nu \in C}
R[\mu,\nu] \, z_C[\nu]
=
\sum_{j=0}^{j<N}
\sum_{x_j \in {B}_j}
\frac{\tau_j^2}{V_j}
K_{j}\!\left( A_j(x_j) - \mu \right)
\sum_{\nu \in C}
\,
K_{j}\!\left( A_j(x_j) - \nu \right)
z_C[\nu]
\end{align}

Crazier Ideas

\begin{align}
Q = -\ln \! \int e^{-L(f)}  P(f) \, df
\end{align}
\begin{align}
\approx -\ln \! \int e^{-L(f)} \, df
= \frac{1}{2}\left(
    \kappa
  + \ln\left| \frac{\mathbf{\Phi}}{2\pi} \right|
  - \mathbf{\Psi}^T
    \mathbf{\Phi}^{-1}
    \mathbf{\Psi}
\right)
\end{align}

PSF Tweaks

\begin{align}
L \equiv
\frac{1}{2} \sum_{j=0}^{j<N}
\frac{1}{V_j}
\sum_{x_j \in {E}_j}
\left(
    z_j[x_j]
  - \tau_{j}
    \sum_{\nu \in C}
    \Bigl[
    \phi_{j}\!\left(
        A_j(x_j) - \nu
    \right)
    +\delta_{j,k}\Delta(A_j(x_j) - \nu)
    \Bigr]
    f(\nu)
\right)^2
\end{align}

Background Matching:

\begin{align}
L \equiv
\frac{1}{2} \sum_{j=0}^{j<N}
\frac{1}{V_j}
\sum_{x_j \in {E}_j}
\left(
    z_j[x_j]
  - \tau_{j}
    b_j
  - \tau_{j}
    \sum_{\nu \in C}
    \phi_{j}\!\left(
        A_j(x_j) - \nu
    \right)
    f(\nu)
\right)^2
+ \Lambda\left(\sum_{j=0}^{j<N}\tau_j b_j\right)^2
\end{align}

\end{document}